\documentclass{article}
\usepackage[utf8]{inputenc}
\usepackage{amsmath}
\usepackage{amssymb}
\usepackage{amsthm}
\usepackage{tikz}
\setlength{\parindent}{0pt}

\newtheorem*{theorem}{Theorem}
\newtheorem*{definition}{Definition}
\newtheorem*{lemma}{Lemma}
\newtheorem*{corollary}{Corollary}
\newtheorem{example}{Example}
\newtheorem{trick}{Trick}
\newtheorem{question}{Question}

\title{Lecture 11: Chain Rule}
\author{}
\date{}

\begin{document}
    
\maketitle

Now with partial derivatives, we can learn more tools to study multivariable 
functions.

\section{Total Differential}

Total differential describes the rate of change of the value of a function in 
terms of all variables.

Suppose there is a function $f(x, y, z)$:
\begin{gather*}
  \begin{split}
    df &= f_xdx + f_ydy + f_zdz \\
       &= \frac{\partial f}{\partial x}dx + \frac{\partial f}{\partial y}dy + \frac{\partial f}{\partial z}dz \\
  \end{split}
\end{gather*}
Notice that $df$ is not a real number, nor is it $\Delta f$. It is an abstract 
notion. So are $dx$, $dy$, and $dz$.

\begin{question}
  What is the intuitive way to understand the total differential formula? It is 
  hard to reason about whether it is valid or not.
\end{question}

How do we use the total differential?
\begin{itemize}
  \item The total differential encodes how changes in independent variables 
    affect the function value.
  \item We can replace $dx$, $dy$, and $dz$ with small variations $\Delta x$, 
    $\Delta y$, and $\Delta z$ to get approximated change of the function value, 
    which is the approximation formula:
    \begin{equation*}
      \Delta f \approx f_x \Delta x + f_y \Delta y + f_z \Delta z
    \end{equation*}
  \item We can divide both sides of the total differential by the differential 
    of a common parameter, such as $dt$, to get the rate of change in terms of 
    this common parameter.
\end{itemize}

\section{Chain Rule}

Actually, the third usage of the total differential described above derives the 
formula of chain rule in multivariable functions.

Suppose there is a function $f(x, y, z)$, and there exists $x = x(t)$, 
$y = y(t)$, and $z = z(t)$, then
\begin{equation*}
  \begin{split}
    \frac{df}{dt} &= f_x \frac{dx}{dt} + f_y \frac{dy}{dt} + f_z \frac{dz}{dt} \\
                  &= \frac{\partial f}{\partial x}\frac{dx}{dt} + \frac{\partial f}{\partial y}\frac{dy}{dt} + \frac{\partial f}{\partial z}\frac{dz}{dt} \\
  \end{split}
\end{equation*}

Why is the formula of chain rule valid?

We can start with the approximation formula. We know that
\begin{equation*}
  \Delta f \approx f_x \Delta x + f_y \Delta y + f_z \Delta z
\end{equation*}
Then we can divide both sides of the equation by a change of the parameter $t$, 
which is $\Delta t$:
\begin{equation*}
  \frac{\Delta f}{\Delta t} \approx f_x \frac{\Delta x}{\Delta t} + f_y \frac{\Delta y}{\Delta t} + f_z \frac{\Delta z}{\Delta t}
\end{equation*}
With $\Delta t \to 0$, according to the definition of derivatives:
\begin{gather*}
  \lim_{\Delta t \to 0}\frac{\Delta f}{\Delta t} = \frac{df}{dt} \\
  \lim_{\Delta t \to 0}\frac{\Delta x}{\Delta t} = \frac{dx}{dt} \\
  \lim_{\Delta t \to 0}\frac{\Delta y}{\Delta t} = \frac{dy}{dt} \\
  \lim_{\Delta t \to 0}\frac{\Delta z}{\Delta t} = \frac{dz}{dt} \\
\end{gather*}
and the approximation becomes more and more accurate. Eventually
\begin{equation*}
  \frac{df}{dt} = f_x \frac{dx}{dt} + f_y \frac{dy}{dt} + f_z \frac{dz}{dt}
\end{equation*}

\begin{example}
  Given that $w = f(x, y, z) = x^2y + z$, $x = t$, $y = e^t$, and $z = \sin t$, 
  find $\frac{dw}{dt}$.

  Solution:

  \begin{gather*}
    \frac{dw}{dt} = f_x \frac{dx}{dt} + f_y \frac{dy}{dt} + f_z \frac{dz}{dt} \\
    f_x = 2xy = 2te^t \\
    f_y = x^2 = t^2 \\
    f_z = 1 \\
    \frac{dx}{dt} = 1 \\
    \frac{dy}{dt} = e^t \\
    \frac{dz}{dt} = \cos t \\
    \begin{split}
      \frac{dw}{dt} &= f_x \frac{dx}{dt} + f_y \frac{dy}{dt} + f_z \frac{dz}{dt} \\
                    &= 2t \cdot e^t \cdot 1 + t^2 \cdot e^t + 1 \cdot \cos t \\
                    &= 2te^t + t^2e^t + \cos t \\
    \end{split} \\
  \end{gather*}

  We can verify the result by first find the formula of $w$ with respect to $t$, 
  and then calculate its derivative:
  \begin{gather*}
    \begin{split}
      w &= x^2y + z \\
        &= t^2e^t + \sin t \\
    \end{split} \\
    \begin{split}
      \frac{dw}{dt} &= \frac{d(t^2e^t + \sin t)}{dt} \\
                    &= 2te^t + t^2e^t + \cos t \\
    \end{split} \\
  \end{gather*}
  The results from the two methods are the same.
\end{example}

We can use chain rule of multivariable functions to derive the product and 
quotient rule of derivatives of single-variable functions:
\begin{itemize}
  \item Product rule:
    \begin{gather*}
      f = u \cdot v \\
      \begin{split}
        \frac{df}{dt} &= \frac{d(u \cdot v)}{dt} \\
                      &= f_u \frac{du}{dt} + f_v \frac{dv}{dt} \\
                      &= \frac{du}{dt} v + u \frac{dv}{dt} \\
      \end{split} \\
    \end{gather*}
  \item Quotient rule:
    \begin{gather*}
      f = \frac{u}{v} \\
      \begin{split}
        \frac{df}{dt} &= \frac{d(\frac{u}{v})}{dt} \\
                      &= f_u \frac{du}{dt} + f_v \frac{dv}{dt} \\
                      &= \frac{1}{v} \cdot \frac{du}{dt} + \frac{-u}{v^2} \cdot \frac{dv}{dt} \\
                      &= \frac{\frac{du}{dt}v - u\frac{dv}{dt}}{v^2} \\
      \end{split} \\
    \end{gather*}
\end{itemize}

\section{Chain Rule with More Variables}

Suppose there is a function $w = f(x, y)$, where $x = x(u, v)$, and 
$y = y(u, v)$, how to find the total differential of $w$ with respect to $u$ and 
$v$?

According to the total differential formula,
\begin{equation*}
  dw = \frac{\partial f}{\partial x}dx + \frac{\partial f}{\partial y}dy
\end{equation*}

\end{document}