\documentclass{article}
\usepackage[utf8]{inputenc}
\usepackage{amsmath}
\usepackage{amssymb}
\usepackage{amsthm}
\usepackage{tikz}
\setlength{\parindent}{0pt}

\newtheorem*{theorem}{Theorem}
\newtheorem*{definition}{Definition}
\newtheorem*{lemma}{Lemma}
\newtheorem*{corollary}{Corollary}
\newtheorem{example}{Example}
\newtheorem{trick}{Trick}
\newtheorem{question}{Question}

\title{Problem Set 2}
\author{}
\date{}

\begin{document}

\begin{center}
{\rmfamily\bfseries\Large 18.02 EXERCISES}

\vspace{25px}

{\rmfamily\bfseries\LARGE Problem Set 2: Matrices and Systems of Equations}
\end{center}

\begin{center}
\section*{Part I}
\end{center}

\subsection*{Unit 1E Equations of Lines and Planes}

1. Find the equations of the following planes: \\
a) through (2, 0, -1) and perpendicular to $\vec{i} + 2\vec{j} - 2\vec{k}$. \\
b) through the origin, (1, 1, 0), and (2, -1, 3) \\
c) through (1, 0, 1), (2, -1, 2), (-1, 3, 2) \\
d) through the points on the $x$, $y$ and $z$-axes where $x = a$, $y = b$, 
$z = c$ respectively (give the equation in the form $Ax + By + Cz = 1$ and 
remember it) \\
e) through (1, 0, 1) and (0, 1, 1) and parallel to $\vec{i} - \vec{j} + 2\vec{k}$

Solution:

a) According to the problem description, the vector $<1, 2, -2>$ is a normal 
vector to the plane. Therefore, the equation of the plane is
\[ x + 2y - 2z = c, \textnormal{where c is a constant} \]
Then we can put the point (2, 0, -1) into the equation:
\[ c = 2 + 2 \times 0 - 2 \times (-1) = 4 \]
Hence, the equation of the plane is 
\[ x + 2y - 2z = 4 \]

b) According to the problem description, two vectors on the plane are
\[ <1, 1, 0>, <2, -1, 3> \]
Therefore, a normal vector to the plane can be calculated as
\begin{gather*}
  \begin{split}
    <1, 1, 0> \times <2, -1, 3> 
    &= \begin{vmatrix}
         \vec{i} & \vec{j} & \vec{k} \\
         1 & 1 & 0 \\
         2 & -1 & 3 \\
       \end{vmatrix} \\
    &= <3, -3, -3> \\
  \end{split}
\end{gather*}
Therefore, the equation of the plane is
\[ 3x - 3y - 3z = c, \textnormal{where c is a constant} \]
Then we can put the point (0, 0, 0) into the equation:
\[ c = 0 \]
Hence the equation of the plane is 
\[ 3x - 3y - 3z = 0 \]

c) According to the problem description, two vectors on the plane are
\[ <1, -1, 1>, <-2, 3, 1> \]
Therefore, a normal vector to the plane can be calculated as
\begin{gather*}
  \begin{split}
    <1, -1, 1> \times <-2, 3, 1> 
    &= \begin{vmatrix}
         \vec{i} & \vec{j} & \vec{k} \\
         1 & -1 & 1 \\
         2 & 3 & 1 \\
       \end{vmatrix} \\
    &= <-4, 1, 5> \\
  \end{split}
\end{gather*}
Therefore, the equation of the plane is
\[ -4x + y + 5z = c, \textnormal{where c is a constant} \]
Then we can put the point (1, 0, 1) into the equation:
\[ c = -4 \times 1 + 0 + 5 \times 1 = 1 \]
Hence the equation of the plane is 
\[ -4x + y + 5z = 1 \]

d) According to the problem description, two vectors on the plane are
\[ <-a, b, 0>, <-a, 0, c> \]
Therefore, a normal vector to the plane can be calculated as
\begin{gather*}
  \begin{split}
    <-a, b, 0> \times <-a, 0, c> 
    &= \begin{vmatrix}
         \vec{i} & \vec{j} & \vec{k} \\
         -a & b & 0 \\
         -a & 0 & c \\
       \end{vmatrix} \\
    &= <bc, ac, ab> \\
  \end{split}
\end{gather*}
Therefore, the equation of the plane is
\[ bcx + acy + abz = k, \textnormal{where k is a constant} \]
Then we can put the point (a, 0, 0) into the equation:
\[ k = bc \cdot a + ac \cdot 0 + ab \cdot 0 = abc \]
Hence the equation of the plane is 
\begin{gather*}
   bcx + acy + abz = abc \\
   \frac{x}{a} + \frac{y}{b} + \frac{z}{c} = 1 \\
\end{gather*}

e) According to the problem description, one vector parallel to the plane can be 
derived from the two points (1, 0, 1) and (0, 1, 1), which is $<-1, 1, 0>$. 
Therefore, a normal vector to the plane can be calculated as
\begin{gather*}
  \begin{split}
    <-1, 1, 0> \times <1, -1, 2> 
    &= \begin{vmatrix}
         \vec{i} & \vec{j} & \vec{k} \\
         -1 & 1 & 0 \\
         1 & -1 & 2 \\
       \end{vmatrix} \\
    &= <2, 2, 0> \\
  \end{split}
\end{gather*}
Therefore, the equation of the plane is 
\[ 2x + 2y = c, \textnormal{where c is a constant} \]
Then we can put the point (1, 0, 1) into the equation:
\[ c = 2 \times 1 + 2 \times 0 = 2 \]
Hence the equation of the plane is
\begin{gather*}
  2x + 2y = 2 \\
  x + y = 1 \\
\end{gather*}

2. Find the dihedral angle between the planes $2x - y + z = 3$ and 
$x + y + 2z = 1$.

Solution:

Suppose that the intersection line between the planes $2x - y + z = 3$ and 
$x + y + 2z = 1$ is $l$. By the definition of dihedral angles, we can find a 
point $O$ on the line $l$, and in the plane $2x - y + z = 3$ find a line 
$OA \perp l$, and in the plane $x + y + 2z = 1$ find a line $OB \perp l$. Then 
the angle $\angle{AOB}$ is the dihedral angle.

Notice that any normal vectors to the plane $2x - y + z = 3$ and the plane 
$x + y + 2z = 1$ are also perpendicular to the line $l$ because $l$ is on both 
planes. Therefore, the vector $\vec{n_1} = <2, -1, 1>$, which is a normal vector 
to the plane $2x - y + z = 3$, and the vector $\vec{n_2} = <1, 1, 2>$, which is 
a normal vector to the plane $x + y + 2z = 1$, are perpendicular to the line $l$.

Therefore, all four vectors $\vec{OA}$, $\vec{OB}$, $\vec{n_1}$, and $\vec{n_2}$ 
are all parallel to the same plane, whose normal vectors are along the line $l$, 
and they form a quadrilateral. Since $\vec{OA} \perp \vec{n_1}$, and 
$\vec{OB} \perp \vec{n_2}$, the angle $\angle{AOB}$ is either equal to or 
supplementary to the angle $\theta$ between two normal vectors $\vec{n_1}$ and 
$\vec{n_2}$.

\begin{gather*}
  \begin{split}
    \cos\theta &= \frac{\vec{n_1} \cdot \vec{n_2}}{|\vec{n_1}||\vec{n_2}|} \\
               &= \frac{3}{\sqrt{6} \times \sqrt{6}} \\
               &= \frac{1}{2} \\
  \end{split} \\
  \theta = \frac{\pi}{3} \\
\end{gather*}
Therefore, the dihedral angle between the two planes are $\frac{\pi}{3}$.

3. Find in parametric form the equations for \\
a) the line through (1, 0, -1) and parallel to $2\vec{i} - \vec{j} + 3\vec{k}$ \\
b) the line through (2, -1, -1) and perpendicular to the plane $x - y + 2z = 3$ \\
c) all lines passing through (1, 1, 1) and lying in the plane $x + 2y - z = 2$

Solution:

a)
\begin{gather*}
  x(t) = 1 + 2t \\
  y(t) = -t \\
  z(t) = -1 + 3t \\
\end{gather*}

b) 
The line is perpendicular to the plane $x - y + 2z = 3$ 
$\iff$ The line is parallel to the normal vectors of the plane $x - y + 2z = 3$
$\iff$ The line is parallel to the vector $<1, -1, 2>$.

Therefore, the parametric equation of the line is
\begin{gather*}
  x(t) = 2 + t \\
  y(t) = -1 - t \\
  z(t) = -1 + 2t \\
\end{gather*}

c)
Since the line is lying in the plane $x + 2y - z = 2$, suppose the line vector 
is $<a, b, c>$, then it satisfies
\begin{gather*}
  <a, b, c> \cdot <1, 2, -1> = 0 \\
  a + 2b - c = 0 \\
  c = a + 2b \\
\end{gather*}
Therefore, the parametric equations of all lines described above are
\begin{gather*}
  x(t) = 1 + at \\
  y(t) = 1 + bt \\
  z(t) = 1 + (a + 2b)t \\
\end{gather*}
where $a$ and $b$ are any constants.

5. The line passing through (1, 1, -1) and perpendicular to the plane 
$x + 2y - z = 3$ intersects the plane $2x - y + z = 1$ at what point?

Solution:

The line is perpendicular to the plane $x + 2y - z = 3$ 
$\iff$ The line is parallel to the normal vectors of the plane $x + 2y - z = 3$
$\iff$ The line is parallel to the vector $<1, 2, -1>$.

Therefore, the parametric equation of the line is
\begin{gather*}
  x(t) = 1 + t \\
  y(t) = 1 + 2t \\
  z(t) = -1 - t \\
\end{gather*}

For the intersection point between the line and the plane, we have
\begin{gather*}
  2x(t) - y(t) + z(t) = 1 \\
  2(1 + t) - (1 + 2t) + (-1 - t) = 1 \\
  t = -1 \\
\end{gather*}
Therefore, the intersection point is $(x(-1), y(-1), z(-1))$, which is 
$(0, -1, 0)$.

6. Show that the distance $D$ from the origin to the plane $ax + by + cz = d$ is 
given by the formula $D = \frac{|d|}{\sqrt{a^2 + b^2 + c^2}}$.

Solution:

We need to find the parametric equation of the line through the origin and 
perpendicular to the plane $ax + by + cz = d$.

The line is perpendicular to the plane $ax + by + cz = d$ 
$\iff$ The line is parallel to the normal vectors of the plane $ax + by + cz = d$
$\iff$ The line is parallel to the vector $<a, b, c>$.

Therefore, the parametric equation of the line is
\begin{gather*}
  x(t) = 0 + at = at \\
  y(t) = 0 + bt = bt \\
  z(t) = 0 + ct = ct \\
\end{gather*}

For the intersection point between the line and the plane, we have
\begin{gather*}
  ax(t) + by(t) + cz(t) = d \\
  a^2t + b^2t + c^2t = d \\
  t = \frac{d}{a^2 + b^2 + c^2} \\
\end{gather*}
Therefore, the intersection point is 
$(\frac{ad}{a^2 + b^2 + c^2}, \frac{bd}{a^2 + b^2 + c^2}, \frac{cd}{a^2 + b^2 + c^2})$

Therefore, the distance $D$ from the origin to the plane is equivalent to the 
distance between these two points:
\begin{gather*}
  \begin{split}
    D &= \sqrt{(\frac{ad}{a^2 + b^2 + c^2})^2 + (\frac{bd}{a^2 + b^2 + c^2})^2 + (\frac{cd}{a^2 + b^2 + c^2})^2)} \\
      &= \sqrt{\frac{(a^2 + b^2 + c^2)d^2}{(a^2 + b^2 + c^2)^2}} \\
      &= \frac{|d|}{\sqrt{a^2 + b^2 + c^2}}
  \end{split}
\end{gather*}

\subsection*{Unit 1F Matrix Algebra}

5. a) Let $A = \begin{pmatrix}
                 0 & 1 \\
                 1 & 1 \\ 
               \end{pmatrix}$. Compute $A^2, A^3$. \\
b) Find $A^2, A^3, A^n$ if $A = \begin{pmatrix}
                                  1 & 1 \\
                                  0 & 1 \\ 
                                \end{pmatrix}$.

Solution:

a) 
\begin{gather*}
  \begin{split}
    A^2 &= \begin{pmatrix}
             0 & 1 \\
             1 & 1 \\ 
           \end{pmatrix} \cdot
           \begin{pmatrix}
             0 & 1 \\
             1 & 1 \\
           \end{pmatrix} \\
        &= \begin{pmatrix}
             1 & 1 \\
             1 & 2 \\ 
           \end{pmatrix} \\
  \end{split} \\
  \begin{split}
    A^3 &= A^2 \cdot A \\
        &= \begin{pmatrix}
             1 & 1 \\
             1 & 2 \\ 
           \end{pmatrix} \cdot
           \begin{pmatrix}
             0 & 1 \\
             1 & 1 \\
           \end{pmatrix} \\
        &= \begin{pmatrix}
             1 & 2 \\
             2 & 3 \\ 
           \end{pmatrix} \\
  \end{split} \\
\end{gather*}

b)
\begin{gather*}
  \begin{split}
    A^2 &= A \cdot A \\
        &= \begin{pmatrix}
             1 & 1 \\
             0 & 1 \\ 
           \end{pmatrix} \cdot
           \begin{pmatrix}
             1 & 1 \\
             0 & 1 \\
           \end{pmatrix} \\
        &= \begin{pmatrix}
             1 & 2 \\
             0 & 1 \\ 
           \end{pmatrix} \\
  \end{split} \\
  \begin{split}
    A^3 &= A^2 \cdot A \\
        &= \begin{pmatrix}
             1 & 2 \\
             0 & 1 \\ 
           \end{pmatrix} \cdot
           \begin{pmatrix}
             1 & 1 \\
             0 & 1 \\
           \end{pmatrix} \\
        &= \begin{pmatrix}
             1 & 3 \\
             0 & 1 \\ 
           \end{pmatrix}
  \end{split} \\
\end{gather*}
The first column in $A$ determines that the first column in $A^{k+1}$ will be 
the same as the first column in $A^k$ where $k$ can be any positive integers.
The second column in $A$ determines that the second column in $A^{k+1}$ will be 
the sum of the first and second columns in $A^k$ where $k$ can be any positive 
integers. Therefore, we can induce that
\begin{gather*}
  A^n = \begin{pmatrix}
          1 & n \\
          0 & 1 \\ 
        \end{pmatrix} \\
\end{gather*}

8. a) If $A \begin{pmatrix}
              1 \\
              0 \\
              0 \\
            \end{pmatrix} = 
            \begin{pmatrix}
              2 \\
              3 \\
              1 \\
            \end{pmatrix}$,
         $A \begin{pmatrix}
              0 \\
              1 \\
              0 \\
            \end{pmatrix} = 
            \begin{pmatrix}
              -1 \\
              0 \\
              4 \\
            \end{pmatrix}$,
         $A \begin{pmatrix}
              0 \\
              0 \\
              1 \\
            \end{pmatrix} = 
            \begin{pmatrix}
              1 \\
              1 \\
              -1 \\
            \end{pmatrix}$, what is the $3 \times 3$ matrix $A$? \\
b) If $A \begin{pmatrix}
           2 \\
           0 \\
           0 \\
         \end{pmatrix} = 
         \begin{pmatrix}
           -2 \\
           0 \\
           4 \\
         \end{pmatrix}$,
      $A \begin{pmatrix}
           1 \\
           1 \\
           1 \\
         \end{pmatrix} = 
         \begin{pmatrix}
           3 \\
           0 \\
           3 \\
         \end{pmatrix}$,
      $A \begin{pmatrix}
           0 \\
           2 \\
           1 \\
         \end{pmatrix} = 
         \begin{pmatrix}
           7 \\
           1 \\
           1 \\
         \end{pmatrix}$, what is the $3 \times 3$ matrix $A$?

Solution:

a) 
According to the definition of matrix product, the result of 
$A \begin{pmatrix}
     1 \\
     0 \\
     0 \\
   \end{pmatrix}$ is the first column of $A$, the result of 
$A \begin{pmatrix}
     0 \\
     1 \\
     0 \\
   \end{pmatrix}$ is the second column of $A$, and the result of 
$A \begin{pmatrix}
     0 \\
     0 \\
     1 \\
   \end{pmatrix}$ is the third column of $A$. Therefore,
\begin{gather*}
  A = \begin{pmatrix}
        2 & -1 & 1 \\
        3 & 0 & 1 \\
        1 & 4 & -1 \\ 
      \end{pmatrix} \\
\end{gather*}

a) (Method 2) 
If we combine the three matrix equations, we can get
\begin{gather*}
  A \cdot \begin{pmatrix}
            1 & 0 & 0 \\
            0 & 1 & 0 \\
            0 & 0 & 1 \\
          \end{pmatrix} =
  \begin{pmatrix}
    2 & -1 & 1 \\
    3 & 0 & 1 \\
    1 & 4 & -1 \\
  \end{pmatrix} \\
  A = \begin{pmatrix}
        2 & -1 & 1 \\
        3 & 0 & 1 \\
        1 & 4 & -1 \\ 
      \end{pmatrix} \cdot
      \begin{pmatrix}
        1 & 0 & 0 \\
        0 & 1 & 0 \\
        0 & 0 & 1 \\
      \end{pmatrix}^{-1} \\
  A = \begin{pmatrix}
        2 & -1 & 1 \\
        3 & 0 & 1 \\
        1 & 4 & -1 \\ 
      \end{pmatrix} \cdot
      \begin{pmatrix}
        1 & 0 & 0 \\
        0 & 1 & 0 \\
        0 & 0 & 1 \\
      \end{pmatrix} \\
  A = \begin{pmatrix}
        2 & -1 & 1 \\
        3 & 0 & 1 \\
        1 & 4 & -1 \\ 
      \end{pmatrix} \\
\end{gather*}

b) (Method 1) 
Suppose $A = \begin{pmatrix}
                  a_1 & a_2 & a_3 \\
                  b_1 & b_2 & b_3 \\
                  c_1 & c_2 & c_3 \\  
                \end{pmatrix}$. Then
\begin{gather*}
  A \begin{pmatrix}
      2 \\
      0 \\
      0 \\
    \end{pmatrix} = 
    \begin{pmatrix}
      -2 \\
      0 \\
      4 \\
    \end{pmatrix} \\
  \begin{pmatrix}
    a_1 & a_2 & a_3 \\
    b_1 & b_2 & b_3 \\
    c_1 & c_2 & c_3 \\
  \end{pmatrix} \cdot 
  \begin{pmatrix}
    2 \\
    0 \\
    0 \\
  \end{pmatrix} = 
  \begin{pmatrix}
    -2 \\
    0 \\
    4 \\
  \end{pmatrix} \\
  \begin{pmatrix}
    2a_1 \\
    2b_1 \\
    2c_1 \\
  \end{pmatrix} = 
  \begin{pmatrix}
    -2 \\
    0 \\
    4 \\
  \end{pmatrix} \\
  a_1 = -1, b_1 = 0, c_1 = 2 \\
\end{gather*}
Also
\begin{gather*}
  A \begin{pmatrix}
      1 \\
      1 \\
      1 \\
    \end{pmatrix} = 
    \begin{pmatrix}
      3 \\
      0 \\
      3 \\
    \end{pmatrix} \\
  \begin{pmatrix}
    a_1 & a_2 & a_3 \\
    b_1 & b_2 & b_3 \\
    c_1 & c_2 & c_3 \\
  \end{pmatrix} \cdot 
  \begin{pmatrix}
    1 \\
    1 \\
    1 \\
  \end{pmatrix} = 
  \begin{pmatrix}
    3 \\
    0 \\
    3 \\
  \end{pmatrix} \\
  \begin{pmatrix}
    a_1 + a_2 + a_3 \\
    b_1 + b_2 + b_3 \\
    c_1 + c_2 + c_3 \\
  \end{pmatrix} = 
  \begin{pmatrix}
    3 \\
    0 \\
    3 \\
  \end{pmatrix} \\
  a_1 + a_2 + a_3 = 3 \\
  b_1 + b_2 + b_3 = 0 \\
  c_1 + c_2 + c_3 = 3 \\
\end{gather*}
And
\begin{gather*}
  A \begin{pmatrix}
      0 \\
      2 \\
      1 \\
    \end{pmatrix} = 
    \begin{pmatrix}
      7 \\
      1 \\
      1 \\
    \end{pmatrix} \\
  \begin{pmatrix}
    a_1 & a_2 & a_3 \\
    b_1 & b_2 & b_3 \\
    c_1 & c_2 & c_3 \\
  \end{pmatrix} \cdot 
  \begin{pmatrix}
    0 \\
    2 \\
    1 \\
  \end{pmatrix} = 
  \begin{pmatrix}
    7 \\
    1 \\
    1 \\
  \end{pmatrix} \\
  \begin{pmatrix}
    2a_2 + a_3 \\
    2b_2 + b_3 \\
    2c_2 + c_3 \\
  \end{pmatrix} = 
  \begin{pmatrix}
    7 \\
    1 \\
    1 \\
  \end{pmatrix} \\
  2a_2 + a_3 = 7 \\
  2b_2 + b_3 = 1 \\
  2c_2 + c_3 = 1 \\
\end{gather*}
Hence we derive the following system of equations:
\begin{gather*}
  \begin{cases}
     a_1 = -1 \\
     b_1 = 0 \\
     c_1 = 2 \\
     a_1 + a_2 + a_3 = 3 \\
     b_1 + b_2 + b_3 = 0 \\
     c_1 + c_2 + c_3 = 3 \\
     2a_2 + a_3 = 7 \\
     2b_2 + b_3 = 1 \\
     2c_2 + c_3 = 1 \\
  \end{cases} \\
\end{gather*}
We can solve this system of equations and get
\begin{gather*}
  A = \begin{pmatrix}
        -1 & 3 & 1 \\
        0 & 1 & -1 \\
        2 & 0 & 1 \\ 
      \end{pmatrix} \\
\end{gather*}

b) (Method 2) 
If we combine the three matrix equations, we can get
\begin{gather*}
  A \cdot \begin{pmatrix}
            2 & 1 & 0 \\
            0 & 1 & 2 \\
            0 & 1 & 1 \\
          \end{pmatrix} =
  \begin{pmatrix}
    -2 & 3 & 7 \\
    0 & 0 & 1 \\
    4 & 3 & 1 \\
  \end{pmatrix} \\
  A = \begin{pmatrix}
        -2 & 3 & 7 \\
        0 & 0 & 1 \\
        4 & 3 & 1 \\ 
      \end{pmatrix} \cdot
      \begin{pmatrix}
        2 & 1 & 0 \\
        0 & 1 & 2 \\
        0 & 1 & 1 \\
      \end{pmatrix}^{-1}
\end{gather*}

9. A square $n \times n$ matrix is called \textbf{orthogonal} if 
$A \cdot A^T = I_n$. Show that this condition is equivalent to saying that \\
a) each row of $A$ is a row vector of length 1. \\
b) two different rows are orthogonal vectors.

Solution:

Suppose $A = \begin{pmatrix}
               a_1 & a_2 & a_3 \\
               b_1 & b_2 & b_3 \\
               c_1 & c_2 & c_3 \\ 
             \end{pmatrix}$, then
$A^T = \begin{pmatrix}
         a_1 & b_1 & c_1 \\
         a_2 & b_2 & c_2 \\
         a_3 & b_3 & c_3 \\ 
       \end{pmatrix}$.
\begin{gather*}
  A \cdot A^T = I_n \\
  \begin{pmatrix}
    a_1 & a_2 & a_3 \\
    b_1 & b_2 & b_3 \\
    c_1 & c_2 & c_3 \\
  \end{pmatrix} \cdot
  \begin{pmatrix}
    a_1 & b_1 & c_1 \\
    a_2 & b_2 & c_2 \\
    a_3 & b_3 & c_3 \\
  \end{pmatrix} = 
  \begin{pmatrix}
    1 & 0 & 0 \\
    0 & 1 & 0 \\
    0 & 0 & 1 \\
  \end{pmatrix} \\
\end{gather*}
Expand the matrix equation, we can derive the following equations:
\begin{gather*}
  a_1^2 + a_2^2 + a_3^3 = 1 \\
  b_1^2 + b_2^2 + b_3^3 = 1 \\
  c_1^2 + c_2^2 + c_3^3 = 1 \\
  a_1b_1 + a_2b_2 + a_3b_3 = 0 \\
  b_1c_1 + b_2c_2 + b_3c_3 = 0 \\
  a_1c_1 + a_2c_2 + a_3c_3 = 0 \\
\end{gather*}
which is equivalent to that each row of $A$ is a row vector of length 1, and two 
different rows in $A$ are orthogonal.

Therefore, the statement in the problem description is proved.

\subsection*{Unit 1G Solving Square Systems; Inverse Matrices}

3. $A = \begin{pmatrix}
          1 & -1 & 1 \\
          0 & 1 & 1 \\
          -1 & -1 & 2 \\
        \end{pmatrix}$, $b = \begin{pmatrix}
                               2 \\
                               0 \\
                               3 \\ 
                             \end{pmatrix}$. Solve $Ax = b$ by finding $A^{-1}$.
                        
Solution:

\begin{gather*}
  Ax = b \\
  x = A^{-1}b \\
  x = \frac{1}{det(A)}adj(A) \cdot b \\
  x = \begin{pmatrix}
        1 & -1 & 1 \\
        0 & 1 & 1 \\
        -1 & -1 & 2 \\ 
      \end{pmatrix}^{-1} \cdot
      \begin{pmatrix}
        2 \\
        0 \\
        3 \\
      \end{pmatrix} \\
  x = \begin{pmatrix}
        \frac{3}{5} & \frac{1}{5} & -\frac{2}{5} \\
        -\frac{1}{5} & \frac{3}{5} & -\frac{1}{5} \\
        \frac{1}{5} & \frac{2}{5} & \frac{1}{5} \\ 
      \end{pmatrix} \cdot
      \begin{pmatrix}
        2 \\
        0 \\
        3 \\
      \end{pmatrix} \\
  x = \begin{pmatrix}
        0 \\
        -1 \\
        1 \\ 
      \end{pmatrix}
\end{gather*}

4. Referring to Exercise 3 above, solve the system 
\[ x_1 - x_2 + x_3 = y_1, x_2 + x_3 = y_2, -x_1 - x_2 + 2x_3 = y_3 \]
for the $x_i$ as functions of the $y_i$.

Solution:

\begin{gather*}
  \begin{cases}
    x_1 - x_2 + x_3 = y_1 \\
    x_2 + x_3 = y_2 \\
    -x_1 - x_2 + 2x_3 = y_3 \\
  \end{cases} \\
  \begin{pmatrix}
    1 & -1 & 1 \\
    0 & 1 & 1 \\
    -1 & -1 & 2 \\
  \end{pmatrix} \cdot
  \begin{pmatrix}
    x_1 \\
    x_2 \\
    x_3 \\
  \end{pmatrix} = 
  \begin{pmatrix}
    y_1 \\
    y_2 \\
    y_3 \\
  \end{pmatrix} \\
  \begin{pmatrix}
    x_1 \\
    x_2 \\
    x_3 \\
  \end{pmatrix} = 
  \begin{pmatrix}
    1 & -1 & 1 \\
    0 & 1 & 1 \\
    -1 & -1 & 2 \\
  \end{pmatrix}^{-1} \cdot
  \begin{pmatrix}
    y_1 \\
    y_2 \\
    y_3 \\
  \end{pmatrix} \\
  \begin{pmatrix}
    x_1 \\
    x_2 \\
    x_3 \\
  \end{pmatrix} = 
  \begin{pmatrix}
    \frac{3}{5} & \frac{1}{5} & -\frac{2}{5} \\
    -\frac{1}{5} & \frac{3}{5} & -\frac{1}{5} \\
    \frac{1}{5} & \frac{2}{5} & \frac{1}{5} \\ 
  \end{pmatrix} \cdot
  \begin{pmatrix}
    y_1 \\
    y_2 \\
    y_3 \\
  \end{pmatrix} \\
  \begin{cases}
    x_1 = \frac{3}{5}y_1 + \frac{1}{5}y_2 - \frac{2}{5}y_3 \\
    x_2 = -\frac{1}{5}y_1 + \frac{3}{5}y_2 - \frac{1}{5}y_3 \\
    x_3 = \frac{1}{5}y_1 + \frac{2}{5}y_2 + \frac{1}{5}y_3 \\ 
  \end{cases} \\
\end{gather*}

5. Show that $(AB)^{-1} = B^{-1}A^{-1}$, by using the definition of inverse 
matrix.

Solution:

By the definition of inverse matrix,
\begin{gather*}
  AB \cdot (AB)^{-1} = I_n \\
  A^{-1}AB \cdot (AB)^{-1} = A^{-1}I_n \\
  B \cdot (AB)^{-1} = A^{-1}I_n \\
  B^{-1}B \cdot (AB)^{-1} = B^{-1}A^{-1}I_n \\
  (AB)^{-1} = B^{-1}A^{-1}I_n \\
  (AB)^{-1} = B^{-1}A^{-1} \\
\end{gather*}

\begin{center}
\section*{Part II}
\end{center}

\end{document}